CleanQ/CleanQ_RBModel.thy
@@ -15,18 +15,419 @@
 section \<open>CleanQ Abstract Ring Buffer Model\<close>
 
 text \<open>
-  We define the CleanQ set model in the the following Isabelle theory: 
+  The second refinement is from unbounded lists to bounded buffer rings for transferring
+  ownership between two agents. As a consequence, the \verb+enqueue+ operation may fail, 
+  because there is no more space in the ring buffer. 
 \<close>
 
 theory CleanQ_RBModel 
 (*<*) imports  
-    "CleanQ_ModularIntervals"
+    CleanQ_ListModel
+    CleanQ_ModularIntervals
 begin
 (*>*)
 
 (* ==================================================================================== *)
 subsection \<open>CleanQ Abstract Ring Buffer Model State\<close>
 (* ==================================================================================== *)
+
+text \<open>
+  We take the state of the CleanQ list model and refine it to use a bounded, circular
+  buffer instead of the lists as transfer sets between the two agents. Again, there is
+  one queue (ring buffer) going from $X$ to $Y$ and another one, for the opposit
+  direction. Expressing the buffers owned by $X$ and $Y$ remain the same. 
+
+  \<^item> rSX: this is the set of buffers owned by X.
+  \<^item> rSY: this is the set of buffers owned by Y.
+  \<^item> rTXY: this is a descriptor ring of buffers in transfer from X to Y.
+  \<^item> rTYX: this is a descriptor ring of buffers in transfer from Y to X.
+\<close>
+
+(* ------------------------------------------------------------------------------------ *)
+subsubsection \<open>Bounded Descriptor Ring\<close>
+(* ------------------------------------------------------------------------------------ *)
+
+text \<open>
+  We first define the type of a the bounded, circular descriptor ring, which we call
+  ring buffer (RB). A ring buffer has a well-defined size, or number of slots, which
+  defines the amount of elements it can hold.  We define the ring buffer as a function
+  from nat to the element. Head and tail define the valid elements in the ring.\<close>
+
+record 'a CleanQ_RB =
+  ring :: "nat \<Rightarrow> 'a"
+  head :: nat
+  tail :: nat
+  size :: nat
+
+text \<open>
+  A ringbuffer has a certain set of valid entries. We now provide definitions to 
+  create the list of entries. Note, this is not [(tail rb) ..<(head rb)]. As there
+  might be a wrap around (e.g. head = 4 tail = 8). We use the nonzero modulus
+  locale to work out the elements.
+\<close>
+
+definition rb_valid_entries :: "'a CleanQ_RB \<Rightarrow> nat list"
+  where "rb_valid_entries rb = (nonzero_modulus.list_between 
+                                       (size rb) (tail rb) (head rb))"
+
+
+text \<open>
+  Using the valid entries, we can define the buffer elements in the descriptor ring
+  by mapping them onto the ring-function of the CleanQ RB:
+\<close>
+
+definition CleanQ_RB_list :: "'a CleanQ_RB \<Rightarrow> 'a list"
+  where "CleanQ_RB_list rb = map (ring rb) (rb_valid_entries rb)"
+
+text \<open>
+  We say a queue is full, if the enqueue operation would lead to the case
+  where the head pointer == tail pointer.
+\<close>
+
+definition rb_full :: "'a CleanQ_RB \<Rightarrow> bool"
+  where "rb_full rb = ((((head rb) + 1) mod (size rb)) = (tail rb))"
+
+definition rb_empty :: "'a CleanQ_RB \<Rightarrow> bool"
+  where "rb_empty rb = ((head rb) = (tail rb))"
+
+
+lemma 
+  assumes sz: "size rb > 1" and  hh: "head rb < size rb" and ll: "tail rb < size rb"
+    shows "rb_empty rb \<longleftrightarrow> rb_valid_entries rb = []"
+proof
+  show "rb_empty rb \<Longrightarrow> rb_valid_entries rb = []"
+  proof -
+    assume e: "rb_empty rb"
+    from e have eq:  "((head rb) = (tail rb))"
+      unfolding rb_empty_def by(simp)
+
+    from sz have nz:
+      "nonzero_modulus (size rb)"
+      by (simp add: nonzero_modulus.intro)
+
+    from eq nz have el:  
+      "(nonzero_modulus.list_between (size rb) (tail rb) (head rb)) = []"
+       using nonzero_modulus.uptol_eq[where N="size rb" and l="tail rb" and h="head rb"]
+       by(auto)
+
+    from el show ?thesis  
+      unfolding rb_valid_entries_def by(simp)
+  qed
+next
+  show "rb_valid_entries rb = [] \<Longrightarrow> rb_empty rb"
+  proof - 
+    assume e: "rb_valid_entries rb = []"
+
+    from sz have nz:
+      "nonzero_modulus (size rb)"
+      by (simp add: nonzero_modulus.intro)    
+
+    from e sz nz have eq:
+      "(tail rb) = (head rb)"
+      unfolding rb_valid_entries_def 
+      using hh ll  nonzero_modulus.uptol_eq_both[where N="size rb" and l="tail rb" and h="head rb"]
+      by(auto)
+
+    from eq show ?thesis 
+      unfolding rb_empty_def by(auto)
+  qed
+qed
+
+
+
+text \<open>
+  We provide functions that increment the head and tail pointers of the queue.
+\<close>
+
+definition rb_incr_head :: "'a CleanQ_RB \<Rightarrow> 'a CleanQ_RB"
+  where "rb_incr_head rb = rb \<lparr> head := ((head rb) + 1) mod (size rb) \<rparr>"
+
+definition rb_incr_tail :: "'a CleanQ_RB \<Rightarrow> 'a CleanQ_RB"
+  where "rb_incr_tail rb = rb \<lparr> tail := ((tail rb) + 1) mod (size rb) \<rparr>"
+
+
+
+
+text \<open>
+  
+\<close>
+
+lemma 
+  assumes notfull: "\<not>(rb_full rb)"  and  hdinc: "rb' = rb \<lparr>   \<rparr>
+
+
+
+
+text \<open>
+  Writing an entry into the ring buffer then corresponds to a function update.
+\<close>
+definition CleanQ_RB_upd :: "nat \<Rightarrow> 'a \<Rightarrow> 'a CleanQ_RB \<Rightarrow> 'a CleanQ_RB"
+  where "CleanQ_RB_upd i b rb = rb \<lparr> ring := (ring rb)(i := b) \<rparr>"
+
+
+
+
+
+
+
+
+
+definition rb_enq :: "'a \<Rightarrow> 'a CleanQ_RB \<Rightarrow> 'a CleanQ_RB" 
+  where "rb_enq b rb = rb \<lparr> ring := (ring rb)((head rb) := b),
+                            head := ((head rb) + 1) mod (size rb) \<rparr>"
+
+definition rb_deq :: "'a CleanQ_RB \<Rightarrow> ('a \<times> 'a CleanQ_RB)"
+  where "rb_deq rb = ((ring rb) (tail rb),  
+                      rb \<lparr> tail := ((tail rb) + 1) mod (size rb) \<rparr> )"
+  
+(*
+
+(* ------------------------------------------------------------------------------------ *)
+subsubsection \<open>System State\<close>
+(* ------------------------------------------------------------------------------------ *)
+
+
+text \<open>
+  We now define the updated system state using \verb+Cleanq_RB+  for the transfer sets
+  between $X$ and $Y$. 
+ \<close>
+
+record 'a CleanQ_RB_State =
+  rSX  :: "'a set"
+  rSY  :: "'a set"
+  rTXY :: "'a CleanQ_RB"
+  rTYX :: "'a CleanQ_RB"
+
+
+text \<open>
+  Like the abstract list model,  we do not specify the representation of the buffer 
+  elements. This can be a single, fixed-sized page frame, a variable-sized base-limit 
+  segment, or a set of memory locations. 
+\<close>
+
+(*<*)
+(* Define some global variables to make Simpl/Complex proofs work *)
+record 'g CleanQ_RB_State_vars = 
+  RingRB_'  :: "nat CleanQ_RB_State"
+(*>*)
+
+
+(* ==================================================================================== *)
+subsection \<open>State Lifting Function\<close>
+(* ==================================================================================== *)
+
+text \<open>
+  The CleanQ RB model is a data refinement of the CleanQ List Model. We can define an
+  interpretation function. That lifts the CleanQ RB model state into the CleanQ
+  list model state by extracting a list of buffers as a subset of the ringbuffer. 
+  We first define a function to convert the ringbuffer representation in to a list, which
+  we use the nonzero_modulus locale to produce a list of indices into the bounded
+  buffer ring and apply them to the \verb+ring+ function of the ringbuffer.
+\<close>
+
+
+text \<open>
+  Then we use this conversion int he state lifting from the RB model to the list model.
+\<close>
+
+definition CleanQ_RB2List :: "'a CleanQ_RB_State  \<Rightarrow> 'a CleanQ_List_State"
+  where "CleanQ_RB2List l = \<lparr> lSX = rSX l, lSY = rSY l, 
+                               lTXY = CleanQ_RB_list (rTXY l), 
+                               lTYX = CleanQ_RB_list (rTYX l) \<rparr>"
+
+
+
+(* ==================================================================================== *)
+subsection \<open>CleanQ RB Model Invariants\<close>
+(* ==================================================================================== *)
+
+text \<open>
+  We now revisit the invariants of the CleanQ list model and specify additional invariants
+  for the CleanQ Ring Buffer model. 
+\<close>
+
+
+(* ------------------------------------------------------------------------------------ *)
+subsubsection \<open>I1: Constant Union (Image)\<close>
+(* ------------------------------------------------------------------------------------ *)
+
+text \<open>
+  The union of all sets is constant. We formulate this as an image for 
+  \verb+CleanQ_List+ where we take the set of the transfer lists and apply the 
+  union.
+\<close>
+
+fun I1_rb_img :: "'a CleanQ_RB_State \<Rightarrow> 'a set \<Rightarrow> bool"
+  where "I1_rb_img rb K \<longleftrightarrow> ((rSX rb) \<union> (rSY rb) 
+                                \<union> set (CleanQ_RB_list (rTXY rb)) 
+                                \<union> set (CleanQ_RB_list (rTYX rb))) = K"
+
+text \<open>
+  We can show that the image of the invariant satisfies the list invariant I1 when
+  we apply the lifting function \verb+CleanQ_RB2List+ to the model state. We prove
+  this in the following lemma.
+\<close>
+
+lemma I1_rb_img_lift:
+  "I1_rb_img R K = I1_list_img (CleanQ_RB2List R) K"
+  unfolding CleanQ_RB2List_def by(simp)
+
+lemma "I1_rb_img R K = I1 (CleanQ_List2Set (CleanQ_RB2List R)) K"
+  unfolding CleanQ_RB2List_def CleanQ_List2Set_def by(simp)
+
+
+(* ------------------------------------------------------------------------------------ *)
+subsubsection \<open>I2: Pairwise Empty (Image)\<close>
+(* ------------------------------------------------------------------------------------ *)
+
+text \<open>
+ All pairwise intersections are empty. Again, we formulate this as an image for
+ \verb+CleanQ_RB+ by extracting the list of buffers from the ring.
+\<close>
+
+fun I2_rb_img :: "'a CleanQ_RB_State \<Rightarrow> bool"
+  where "I2_rb_img rb \<longleftrightarrow> rSX rb \<inter> rSY rb = {} 
+           \<and> rSX rb \<inter> set (CleanQ_RB_list (rTXY rb)) = {} 
+           \<and> rSX rb \<inter> set (CleanQ_RB_list (rTYX rb)) = {} 
+           \<and> rSY rb \<inter> set (CleanQ_RB_list (rTXY rb)) = {} 
+           \<and> rSY rb \<inter> set (CleanQ_RB_list (rTYX rb)) = {} 
+           \<and> set (CleanQ_RB_list (rTXY rb)) \<inter> set (CleanQ_RB_list (rTYX rb)) = {}"
+
+
+text \<open>
+  Finally, we can show that the image of the Invariant I2 is equivalent to the list 
+  version of this invariant, when we lift the CleanQ RB State to the CleanQ List State. 
+  We prove this in the following lemma:
+\<close>
+
+lemma I2_rb_img_lift:
+  "I2_rb_img R = I2_list_img (CleanQ_RB2List R)"
+  unfolding CleanQ_RB2List_def by(simp)
+
+
+lemma "I2_rb_img R = I2 (CleanQ_List2Set (CleanQ_RB2List R))"
+  unfolding CleanQ_RB2List_def CleanQ_List2Set_def by(simp)
+
+
+(* ------------------------------------------------------------------------------------ *)
+subsubsection \<open>I3: Distinct Transferlists\<close>
+(* ------------------------------------------------------------------------------------ *)
+
+text \<open>
+  Next we provide an interpretation of the I3 invariant in the ring buffer representation. 
+\<close>
+
+fun I3_rb_img :: "'a CleanQ_RB_State \<Rightarrow> bool"
+  where "I3_rb_img st_list \<longleftrightarrow> distinct (CleanQ_RB_list (rTXY st_list)) 
+                             \<and> distinct (CleanQ_RB_list (rTYX st_list))"
+
+
+lemma I3_rb_img_lift:
+  "I3_rb_img R = I3 (CleanQ_RB2List R)"
+  unfolding CleanQ_RB2List_def by(simp)
+
+
+(* ------------------------------------------------------------------------------------ *)
+subsubsection \<open>All CleanQ RB Invariants\<close>
+(* ------------------------------------------------------------------------------------ *)
+
+text \<open>
+  We combine all invariants for the abstract CleanQ RB model and define the unified 
+  predicate \verb+CleanQ_RB_Invariants+.
+\<close>
+
+fun CleanQ_RB_Invariants :: "'a set \<Rightarrow> 'a CleanQ_RB_State \<Rightarrow> bool"
+  where "CleanQ_RB_Invariants K rb \<longleftrightarrow> I1_rb_img rb K \<and> I2_rb_img rb \<and> I3_rb_img rb"
+
+
+text \<open>
+  Finally, we can show that when the CleanQ RB invariants are satisfied, this also
+  satisfies the set invariants.
+\<close>
+
+lemma CleanQ_RB_Invariants_List_Invariants:
+  "CleanQ_RB_Invariants K L \<Longrightarrow> CleanQ_List_Invariants K (CleanQ_RB2List L)"
+  unfolding CleanQ_RB2List_def by simp
+
+
+(* ==================================================================================== *)
+subsection \<open>State Transition Operations\<close>
+(* ==================================================================================== *)
+
+text \<open>
+  We now formulate the state transition operations in terms of the CleanQ RB model
+  state. Again, the two agents can, independently from each other, perform one of 
+  two operations, \verb+enqueue+ and \verb+dequeue+,  which trigger an ownership 
+  transfer of buffer elements.  
+\<close>
+
+(* ------------------------------------------------------------------------------------ *)
+subsubsection \<open>Enqueue Operation\<close>
+(* ------------------------------------------------------------------------------------ *)
+
+text \<open>
+  The \verb+enqueue+ operation is analogous to the List operations except that the elements
+  are written into a slot in the descriptor ring and then the pointers adapted accordingly. 
+\<close>
+
+definition CleanQ_RB_enq_x :: "'a \<Rightarrow> 'a CleanQ_RB_State  \<Rightarrow> 'a CleanQ_RB_State"
+  where "CleanQ_RB_enq_x b rb = rb \<lparr> rSX := (rSX rb) - {b}, rTXY := rb_enq b (rTXY rb) \<rparr>"
+
+definition CleanQ_RB_enq_y :: "'a \<Rightarrow> 'a CleanQ_RB_State  \<Rightarrow> 'a CleanQ_RB_State"
+  where "CleanQ_RB_enq_y b rb = rb \<lparr> rSY := (rSY rb) - {b}, rTYX := rb_enq b (rTYX rb) \<rparr>"
+
+
+
+lemma 
+  assumes notfull : "\<not> rb_full rb" and pos: "i = (head rb)"
+  shows "(ring (rb_enq b rb)) i = b"
+  using notfull pos unfolding rb_enq_def by(simp)
+
+
+lemma
+  assumes notfull : "\<not> rb_full rb" and dist: "b \<notin> set (CleanQ_RB_list rb)"
+  shows "set (CleanQ_RB_list rb) \<subset> set (CleanQ_RB_list (rb_enq b rb))"
+  using notfull dist unfolding rb_enq_def CleanQ_RB_list_def 
+  apply(simp)
+  
+  
+  sorry
+    
+ 
+
+
+(*
+
+
+lemma 
+ assumes notfull : "\<not> rb_full rb"  and  pos: "i = (head rb)"
+   shows "CleanQ_RB_list (rb_enq b rb) = (CleanQ_RB_list rb) @ [b]"
+  unfolding CleanQ_RB_list_def rb_enq_def 
+proof (simp)
+
+  have "map ((ring rb)(head rb := b))
+     (nonzero_modulus.list_between (size rb) (tail rb)
+       (Suc (head rb) mod size rb)) =
+     map  ((ring rb)(head rb := b))
+     (nonzero_modulus.list_between (size rb) (tail rb)
+       (head rb)) @
+    []"
+    apply(simp) 
+    
+
+
+
+qed
+  
+
+
+lemma CleanQ_RB_enq_x_equal :
+  assumes notfull : "\<not> rb_full (rTXY rb)"
+    shows "CleanQ_RB2List (CleanQ_RB_enq_x b rb) = CleanQ_List_enq_x b (CleanQ_RB2List rb)"
+  unfolding CleanQ_RB2List_def CleanQ_RB_enq_x_def CleanQ_List_enq_x_def rb_enq_def CleanQ_RB_list_def
+  apply(simp)
+
+(*
 
 text \<open>
   The third refinement is trying to get as close to the C implementation as possible.
@@ -166,5 +567,5 @@ fun CleanQ_RB_Invariants :: "'a set \<Rightarrow> 'a CleanQ_RB_State \<Rightarro
   where "CleanQ_RB_Invariants K rb \<longleftrightarrow> I1_img rb K \<and> I2_img rb \<and> I3_img rb \<and> I4 rb \<and> I5 rb"
 
 end (*Modulus end *)
-
+*)
 end
